proof/format_proof.v
@@ -5,440 +5,9 @@ Require Import VST.floyd.library.
 Require Import printer.printer_files.compiled_format.
 Require Import printer.verified_printer.Format.
 Require Import Coq.Strings.Ascii.
+Require Import format_specs.
+Require Import format_std_proof.
 
-Instance CompSpecs : compspecs. make_compspecs prog. Defined.
-Definition Vprog : varspecs. mk_varspecs prog. Defined.
-
-Definition max_spec : ident * funspec := 
-DECLARE _max
-  WITH a : Z, b : Z
-  PRE [ tuint, tuint ]
-    PROP (
-      0 <= a <= Int.max_unsigned;
-      0 <= b <= Int.max_unsigned
-    )
-    PARAMS (Vint (Int.repr a); Vint (Int.repr b))
-    SEP ()
-  POST [ tuint ] EX q : Z,
-    PROP (q = Z.max a b) 
-    RETURN (Vint (Int.repr q)) 
-    SEP().
-    
-Definition strlen_spec :=
- DECLARE _strlen
-  WITH sh: share, s : list byte, str: val
-  PRE [ tptr tschar ]
-    PROP (readable_share sh)
-    PARAMS (str)
-    SEP (cstring sh s str)
-  POST [ size_t ]
-    PROP ()
-    RETURN (Vptrofs (Ptrofs.repr (Zlength s)))
-    SEP (cstring sh s str).
-
-Definition strcpy_spec :=
- DECLARE _strcpy
-  WITH wsh: share, rsh: share, dest : val, n : Z, src : val, s : list byte
-  PRE [ tptr tschar, tptr tschar ]
-    PROP (writable_share wsh; readable_share rsh; Zlength s < n)
-    PARAMS (dest; src)
-    SEP (data_at_ wsh (tarray tschar n) dest; cstring rsh s src)
-  POST [ tptr tschar ]
-    PROP ()
-    RETURN (dest)
-    SEP (cstringn wsh s n dest; cstring rsh s src).
-
-Definition strcat_spec :=
- DECLARE _strcat
-  WITH wsh: share, rsh: share, dest : val, n : Z, src : val, b : list byte, s : list byte
-  PRE [ tptr tschar, tptr tschar ]
-    PROP (writable_share wsh; readable_share rsh; Zlength b + Zlength s < n)
-    PARAMS (dest; src)
-    SEP (cstringn wsh b n dest; cstring rsh s src)
-  POST [ tptr tschar]
-    PROP ()
-    RETURN (dest)
-    SEP (cstringn wsh (b ++ s) n dest; cstring rsh s src).
-
-Definition t_list := Tstruct _list noattr.
-
-Fixpoint listrep (sigma: list (Z * (list byte))) (p: val) : mpred :=
- match sigma with
- | (a, b)::hs =>
-    EX x:val, EX y: val,
-    (emp || malloc_token Ews (Tarray tschar (Zlength b + 1) noattr) y) *
-    cstring Ews b y *
-    malloc_token Ews t_list p * 
-    data_at Ews t_list ((Vint (Int.repr a), (y, x)) : @reptype CompSpecs t_list) p *
-    listrep hs x
- | nil =>
-    !! (p = nullval) && emp
- end.
-
-Fixpoint lseg (sigma: list (Z * (list byte))) (x z: val) : mpred :=
-  match sigma with
-  | nil => !! (x = z) && emp
-  | (a, b)::hs => EX h: val, EX y:val, 
-        (emp || malloc_token Ews (Tarray tschar (Zlength b + 1) noattr) y) *
-        cstring Ews b y *
-        malloc_token Ews t_list x * 
-        data_at Ews t_list ((Vint (Int.repr a)), (y, h)) x * 
-        lseg hs h z
-  end.
-
-Arguments lseg sigma x z : simpl never.
-
-Definition list_copy_spec : ident * funspec :=
-DECLARE _list_copy
-  WITH sh : share, l : val, sigma : list (Z * (list byte)), gv: globals
-  PRE [ tptr t_list ]
-    PROP(0 <= Zlength sigma <= Int.max_unsigned;
-         Forall (fun x => 0 <= (fst x) <= Int.max_unsigned /\ 0 <= Zlength (snd x) + 1 <= Int.max_unsigned) sigma)
-    PARAMS(l) GLOBALS(gv)
-    SEP(listrep sigma l; mem_mgr gv)
-  POST [ tptr t_list ] 
-    EX q: val,
-    PROP()
-    RETURN(q)
-    SEP(listrep sigma l; listrep sigma q; mem_mgr gv).
-
-
-Definition t_format := Tstruct _t noattr.
-
-Fixpoint string_to_list_byte (s: string) : list byte :=
-  match s with
-  | EmptyString => nil
-  | String a s' => Byte.repr (Z.of_N (Ascii.N_of_ascii a))
-                                      :: string_to_list_byte s'
-  end.
-
-Fixpoint text_from (sigma : list (Z * list byte)) : list byte :=
-  match sigma with 
-  | nil => nil
-  | (s, l)::hs => (repeat (Byte.repr (Z.of_N 32)) (Z.to_nat s) ) ++ l ++ text_from hs
-end.
-
-Definition to_text_eq (to_text : nat -> string -> string) (sigma : list (Z * list byte)) :=
-  string_to_list_byte (to_text (Z.to_nat 0) EmptyString) = text_from sigma.
-
-Record list_mp (sigma : list (Z * list byte)) : Prop :=
-  mk_list_mp {
-    list_mp_length     : 0 <= Zlength sigma + 1 <= Int.max_unsigned;
-    list_mp_forall_fst :
-      Forall (fun x => 0 <= (fst x) <= Int.max_unsigned) sigma;
-    list_mp_forall_snd :
-      Forall (fun x => 0 <= Zlength (snd x) + 1 <= Int.max_unsigned) sigma;
-  }.
-
-(* Definition list_mp (sigma : list (Z * list byte)) : Prop :=
-  << list_mp_length     : 0 <= Zlength sigma + 1 <= Int.max_unsigned >> /\
-  << list_mp_forall_fst :
-      Forall (fun x => 0 <= (fst x) <= Int.max_unsigned) sigma >> /\
-  << list_mp_forall_snd :
-      Forall (fun x => 0 <= Zlength (snd x) + 1 <= Int.max_unsigned) sigma >>. *)
-
-Definition mformat (G : t) (x : val) : mpred := 
-  EX sigma : list (Z * list byte),
-  EX p : val,
-  !! (to_text_eq G.(to_text) sigma) &&
-  !! (list_mp sigma) &&
-  !! (<< HGMU  : 0 <= Z.of_nat (height G) <= Int.max_unsigned >>) &&
-  !! (<< FLWMU : 0 <= Z.of_nat (first_line_width G) <= Int.max_unsigned >>) &&
-  !! (<< MWMU  : 0 <= Z.of_nat (middle_width G) <= Int.max_unsigned >>) &&
-  !! (<< LLWMU : 0 <= Z.of_nat (last_line_width G) <= Int.max_unsigned >>) &&
-  malloc_token Ews t_format x * 
-  data_at Ews t_format (Vint (Int.repr (Z.of_nat G.(height))),
-                        (Vint (Int.repr (Z.of_nat G.(first_line_width))),
-                         (Vint (Int.repr (Z.of_nat G.(middle_width))),
-                          (Vint (Int.repr (Z.of_nat G.(last_line_width))), p)))) x *
-  listrep sigma p
- .
-
- Definition concrete_mformat (G : t) (x : val) (sigma : list (Z * list byte)) (p : val) : mpred :=
-  !! (to_text_eq G.(to_text) sigma) &&
-  !! (list_mp sigma) &&
-  !! (0 <= Z.of_nat (height G) <= Int.max_unsigned) &&
-  !! (0 <= Z.of_nat (first_line_width G) <= Int.max_unsigned) &&
-  !! (0 <= Z.of_nat (middle_width G) <= Int.max_unsigned) &&
-  !! (0 <= Z.of_nat (last_line_width G) <= Int.max_unsigned) &&
-  sepcon (malloc_token Ews t_format x)
-  (sepcon 
-  (data_at Ews t_format (Vint (Int.repr (Z.of_nat G.(height))),
-                        (Vint (Int.repr (Z.of_nat G.(first_line_width))),
-                         (Vint (Int.repr (Z.of_nat G.(middle_width))),
-                          (Vint (Int.repr (Z.of_nat G.(last_line_width))), p)))) x)
-  (listrep sigma p))
-.
-
-
- Definition less_components_spec : ident * funspec :=
- DECLARE _less_components
-  WITH p : val, G : t, q : val, G' : t
-  PRE [ tptr t_format, tptr t_format]
-    PROP()
-    PARAMS(p; q)
-    SEP(mformat G p; mformat G' q)
-  POST [ tbool ]
-    EX a : bool,
-    PROP(a = less_components G G')
-    RETURN(Val.of_bool a)
-    SEP(mformat G p; mformat G' q).
-
-
-Definition is_less_than_spec : ident * funspec :=
-DECLARE _is_less_than
-  WITH p : val, G : t, q : val, G' : t
-  PRE [ tptr t_format, tptr t_format]
-    PROP()
-    PARAMS(p; q)
-    SEP(mformat G p; mformat G' q)
-  POST [ tbool ]
-    EX a : bool,
-    PROP(a = is_less_than G G')
-    RETURN(Val.of_bool a)
-    SEP(mformat G p; mformat G' q).
-
-
-Definition empty_spec : ident * funspec :=
-DECLARE _empty 
-  WITH gv : globals
-  PRE []
-    PROP()
-    PARAMS() GLOBALS(gv)
-    SEP(mem_mgr gv)
-  POST [ tptr t_format ]
-    EX p : val,
-    PROP()
-    RETURN(p)
-    SEP(mem_mgr gv; mformat empty p).
-
-
-Fixpoint list_byte_to_string (sigma: list byte) : string :=
-  match sigma with 
-  | nil => EmptyString
-  | (h :: hs) => String (Ascii.ascii_of_N (Z.to_N (Byte.unsigned h))) (list_byte_to_string hs)
-  end.
-
-
-Definition line_spec : ident * funspec :=
-DECLARE _line
-  WITH p : val, sigma : list byte, gv : globals
-  PRE [ tptr tschar ]
-    PROP(0 <= Zlength sigma + 1 <= Int.max_unsigned)
-    PARAMS(p) GLOBALS(gv)
-    SEP(mem_mgr gv; cstring Ews sigma p)
-  POST [ tptr t_format ]
-    EX q : val,
-    PROP()
-    RETURN(q)
-    SEP(mem_mgr gv; mformat (line (list_byte_to_string sigma)) q).
-    
-
-Definition sp_spec : ident * funspec :=
-DECLARE _sp
-  WITH n : Z, gv : globals
-  PRE [ size_t ]
-    PROP (0 <= n <= Int.max_unsigned)
-    PARAMS(Vptrofs (Ptrofs.repr n)) GLOBALS(gv)
-    SEP(mem_mgr gv)
-  POST [ tptr tschar ]
-    EX p : val,
-    PROP()
-    RETURN(p)
-    SEP(cstring Ews (string_to_list_byte (sp (Z.to_nat n))) p;
-         malloc_token Ews (Tarray tschar (n + 1) noattr) p; mem_mgr gv).
-
-Definition add_above_spec : ident * funspec :=
-DECLARE _add_above
-  WITH G : t, F : t, pointer_G : val, pointer_F : val, gv : globals
-  PRE [ tptr t_format, tptr t_format ]
-    PROP ()
-    PARAMS(pointer_G; pointer_F) GLOBALS(gv)
-    SEP(mformat G pointer_G; mformat F pointer_F; mem_mgr gv)
-  POST [ tptr t_format ]
-    EX p : val,
-    PROP()
-    RETURN(p)
-    SEP(mformat G pointer_G; mformat F pointer_F; 
-        mformat (add_above G F) p; mem_mgr gv).
-
-(* ================================================================= *)
-
-
-Definition Gprog : funspecs :=
-        ltac:(with_library prog [
-                   max_spec; strlen_spec; strcpy_spec; strcat_spec;
-                   list_copy_spec; less_components_spec; is_less_than_spec; 
-                   empty_spec; line_spec; sp_spec
- ]).
-
-(* ================================================================= *)
-
-Lemma body_max: semax_body Vprog Gprog f_max max_spec.
-Proof.
-  start_function. 
-  forward_if.
-  { forward. Exists b. entailer!. }
-  forward. Exists a. entailer!.
-Qed.
-
-Lemma body_strlen: semax_body Vprog Gprog f_strlen strlen_spec.
-Proof.
-start_function.
-unfold cstring in *.
-Intros.
-forward.
-
-forward_loop  (EX i : Z,
-  PROP (0 <= i < Zlength s + 1)
-  LOCAL (temp _str str; temp _i (Vptrofs (Ptrofs.repr i)))
-  SEP (data_at sh (tarray tschar (Zlength s + 1))
-          (map Vbyte (s ++ [Byte.zero])) str)).
-
-{ Exists 0. entailer. }
-Intros i. forward. forward_if. forward. entailer!. 
-repeat f_equal. cstring.
-forward. entailer. Exists (i + 1). entailer!.
-assert(0 <= i + 1 < Zlength (s ++ [Byte.zero])).
-{ assert (i < Zlength s) by cstring.
-  autorewrite with sublist.
-  cstring. }
-autorewrite with sublist in H6. simpl in H6.
-apply H6.
-Qed.
-
-Lemma body_strcpy : semax_body Vprog Gprog f_strcpy strcpy_spec.
-Proof.
-start_function.
-
-unfold cstring,cstringn in *.
-forward.
-Intros.
-forward_loop (EX i : Z,
-  PROP (0 <= i < Zlength s + 1)
-  LOCAL (temp _i (Vptrofs (Ptrofs.repr i)); temp _dest dest; temp _src src)
-  SEP (data_at wsh (tarray tschar n)
-        (map Vbyte (sublist 0 i s) ++ Zrepeat Vundef (n - i)) dest;
-       data_at rsh (tarray tschar (Zlength s + 1)) (map Vbyte (s ++ [Byte.zero])) src)).
-{ Exists 0. entailer. }
-Intros i. forward. forward. forward. forward_if.
-{ forward. entailer!. apply derives_refl'. f_equal.
-  rewrite upd_Znth_app2.
-  2: { list_solve. }
-  assert (i - Zlength (map Vbyte (sublist 0 i s)) = 0) as AA by list_solve.
-  rewrite AA. unfold Zrepeat.
-  remember (Z.to_nat (n - i)). destruct n0.
-  { lia. }
-  simpl. 
-  assert (i = Zlength s) by cstring.
-  replace (Z.to_nat (n - (Zlength s + 1))) with n0 by lia.
-  list_solve. }
-forward. Exists (i + 1). entailer!. 
-2: { rewrite upd_Znth_app2.
-     all: list_solve. }
-assert (0 <= i + 1 < (Zlength (s ++ [Byte.zero]))) as AA.
-{ assert (i < Zlength s) as LT by cstring.
-  autorewrite with sublist.
-  cstring. }
-autorewrite with sublist in AA. simpl in AA.
-apply AA.
-Qed.
-
-Lemma body_strcat: semax_body Vprog Gprog f_strcat strcat_spec.
-Proof.
-  leaf_function.
-  start_function.
-  unfold cstringn, cstring in *.
-  forward.
-  forward_loop(
-    EX i : Z,
-    PROP (0 <= i < Zlength b + 1)
-    LOCAL (temp _i (Vptrofs (Ptrofs.repr i)); temp _dest dest; temp _src src)
-    SEP (cstringn wsh b n dest; cstring rsh s src))
-  break:
-  (
-    PROP ()
-    LOCAL (temp _i (Vptrofs (Ptrofs.repr (Zlength b))); temp _dest dest; temp _src src)
-    SEP (cstringn wsh b n dest; cstring rsh s src)).
-  { Exists 0. unfold cstringn, cstring. entailer!. }
-  {
-    unfold cstringn, cstring.
-    Intros i.
-    forward. 
-    { entailer!. }
-    { entailer!. list_solve. }
-    autorewrite with sublist norm.
-    forward.
-    forward_if.
-    { forward. unfold cstringn, cstring. entailer!. do 2 f_equal. list_solve. }
-    forward.
-    Exists (i + 1).
-    unfold cstringn, cstring.
-    entailer!.
-    list_solve.
-  }
-  unfold cstringn, cstring.
-  forward.
-  autorewrite with sublist norm in *.
-  forward_loop(
-    EX j : Z,
-    PROP (0 <= j < Zlength s + 1)
-    LOCAL (temp _i (Vptrofs (Ptrofs.repr (Zlength b)));
-            temp _j (Vptrofs (Ptrofs.repr j));
-            temp _dest dest; temp _src src)
-    SEP ( data_at wsh (tarray tschar n) (map Vbyte (b ++ sublist 0 j s) ++ 
-    Zrepeat Vundef (n - (Zlength b + j))) dest;
-        cstring rsh s src)
-  ).
-  { Exists 0. unfold cstring, cstringn. autorewrite with sublist norm. entailer!. list_solve. }
-  { 
-    Intros j.
-    unfold cstringn, cstring.
-    autorewrite with sublist norm in *.
-    Intros.
-    do 3 forward.
-    { entailer!. }
-    forward_if.
-    { forward. autorewrite with sublist norm. entailer!; list_solve. }
-    forward.
-    Exists (j + 1).
-    entailer!.
-    { list_solve. }
-    unfold cstringn, cstring.
-    autorewrite with sublist norm.
-    entailer!.
-    list_solve.
-  }
-Qed.
-
-Arguments listrep sigma p : simpl never.
-
-Lemma listrep_local_facts:
-  forall sigma p,
-   listrep sigma p |--
-   !! (is_pointer_or_null p /\ (p=nullval <-> sigma=nil)).
-Proof.
-  intros.
-
-  revert p; induction sigma; intros p.
-  { unfold listrep. entailer!. split; auto. }
-  unfold listrep; fold listrep. destruct a. entailer. entailer!. split; intro.
-  2: now inversion H4.
-  subst p. eapply field_compatible_nullval; eauto.
-Qed.
-#[export] Hint Resolve listrep_local_facts : saturate_local.
-
-Lemma listrep_valid_pointer:
-  forall sigma p,
-   listrep sigma p |-- valid_pointer p.
-Proof.
-intros.
-unfold listrep. destruct sigma; simpl.
-{ entailer!. }
-destruct p0. Intros x y. auto with valid_pointer.
-Qed.
-#[export] Hint Resolve listrep_valid_pointer : valid_pointer.
-  
 Lemma less_components_fact1: 
   forall (x y : nat), 
     (0 <= (Z.of_nat x) <= Int.max_unsigned) ->
@@ -450,41 +19,40 @@ Proof.
   f_equal.
   remember (Z.of_nat x <=? Z.of_nat y) as comp.
   destruct comp.
-  + remember (Z.of_nat y) as Y.
+  { remember (Z.of_nat y) as Y.
     remember (Z.of_nat x) as X.
-    assert (X <= Y \/  X > Y). lia.
-    destruct H1. {
-      remember (Int.ltu (Int.repr Y) (Int.repr X)).
+    assert (X <= Y \/  X > Y) as AA. lia.
+    destruct AA. 
+    { remember (Int.ltu (Int.repr Y) (Int.repr X)) as b eqn:AA.
       destruct b.
-      symmetry in Heqb.
-      apply ltu_inv in Heqb.
-      repeat rewrite Int.unsigned_repr in Heqb by auto.
+      symmetry in AA.
+      apply ltu_inv in AA.
+      repeat rewrite Int.unsigned_repr in AA by auto.
       all: lia.
-    } {
-      remember (Int.ltu (Int.repr Y) (Int.repr X)).
-      destruct b.
-      - destruct (Z.leb_spec0 X Y); lia.
-      - lia.
-    }
-  + remember (Z.of_nat y) as Y.
-    remember (Z.of_nat x) as X.
-    assert (X <= Y \/  X > Y). lia.
-    destruct H1. {
-      remember (Int.ltu (Int.repr Y) (Int.repr X)).
-      destruct b. lia.
-      symmetry in Heqb.
-      apply ltu_false_inv in Heqb.
-      repeat rewrite Int.unsigned_repr in Heqb by auto.
-      destruct (Z.leb_spec0 X Y).
-      lia. lia.
-    } {
-      remember (Int.ltu (Int.repr Y) (Int.repr X)).
-      destruct b. lia.
-      symmetry in Heqb.
-      apply ltu_false_inv in Heqb.
-      repeat rewrite Int.unsigned_repr in Heqb by auto.
-      lia.
-    }
+    } 
+    remember (Int.ltu (Int.repr Y) (Int.repr X)).
+    destruct b.
+    2: now lia.
+    destruct (Z.leb_spec0 X Y); lia.
+    
+  }
+  remember (Z.of_nat y) as Y.
+  remember (Z.of_nat x) as X.
+  assert (X <= Y \/  X > Y) as AA. lia.
+  destruct AA. 
+  { remember (Int.ltu (Int.repr Y) (Int.repr X)) as b eqn:AA.
+    destruct b. lia.
+    symmetry in AA.
+    apply ltu_false_inv in AA.
+    repeat rewrite Int.unsigned_repr in AA by auto.
+    destruct (Z.leb_spec0 X Y); lia.
+  } 
+  remember (Int.ltu (Int.repr Y) (Int.repr X)) as b eqn:AA.
+  destruct b. lia.
+  symmetry in AA.
+  apply ltu_false_inv in AA.
+  repeat rewrite Int.unsigned_repr in AA by auto.
+  lia.
 Qed.
   
 Lemma less_components_fact2:
@@ -493,111 +61,105 @@ Lemma less_components_fact2:
 Proof.
   intros.
   destruct (Nat.leb_spec0 x y).
-  - apply inj_le in l.
+  { apply inj_le in l.
     destruct (Z.leb_spec0 (Z.of_nat x) (Z.of_nat y)); auto.
-  - destruct (Z.leb_spec0 (Z.of_nat x) (Z.of_nat y)); auto.
-    apply Nat2Z.inj_le in l. lia.
+  }
+  destruct (Z.leb_spec0 (Z.of_nat x) (Z.of_nat y)); auto.
+  apply Nat2Z.inj_le in l. lia.
 Qed.
 
 Lemma body_less_components: semax_body Vprog Gprog f_less_components less_components_spec.
 Proof.
   start_function.
   unfold mformat.
-  Intros sigmaG pG.
-  Intros sigmaG' pG'.
-  forward.
-  forward.
+  Intros sigmaG pG sigmaG' pG'.
+  do 2 forward. 
+  getnw. rename FMT_MP into FMT_MP'. getnw.
+  destruct FMT_MP, FMT_MP'.
   forward_if(
     EX t1: bool,
-    PROP(t1 = andb 
-    ((Z.of_nat (height G)) <=? Z.of_nat (height G'))
-    ((Z.of_nat (first_line_width G)) <=? Z.of_nat (first_line_width G'))
+    PROP(<< first_comp_eq : t1 = andb 
+      ((Z.of_nat (height G)) <=? Z.of_nat (height G'))
+      ((Z.of_nat (first_line_width G)) <=? Z.of_nat (first_line_width G')) >> 
     )
     LOCAL(temp _t'1 (Val.of_bool t1); temp _G p; temp _F q)
     SEP(
-          concrete_mformat G p sigmaG pG;
-          concrete_mformat G' q sigmaG' pG'
+      concrete_mformat G p sigmaG pG;
+      concrete_mformat G' q sigmaG' pG'
     )
-  ). {
-  do 3 forward.
-  Exists ((Z.of_nat (first_line_width G)) <=? (Z.of_nat (first_line_width G'))).
-  unfold mformat.
-  entailer!.
-  + apply less_components_fact1; auto.
-  + unfold concrete_mformat. entailer!.
-  } {
-  forward.
-  Exists false.
-  entailer.
-  unfold concrete_mformat.
-  entailer!.
+  ). 
+
+  { do 3 forward.
+    Exists ((Z.of_nat (first_line_width G)) <=? (Z.of_nat (first_line_width G'))).
+    unfold concrete_mformat. 
+    unnw. entailer!. split.
+    { apply less_components_fact1; auto. }
+    { split; apply mk_format_mp; auto. }
+  }
+  { forward.
+    Exists false.
+    unfold concrete_mformat. unnw.
+    entailer!.
+    { split; apply mk_format_mp; auto. }
   }
 
-  Intros first_two_comp.
+  Intros first_comp.
   forward_if(
     EX t2: bool,
-    PROP(t2 = andb first_two_comp 
+    PROP(<< second_comp_eq : t2 = andb first_comp 
       (((Z.of_nat (middle_width G))) <=?
-      (Z.of_nat (middle_width G'))))
+      (Z.of_nat (middle_width G'))) >>)
     LOCAL(temp _t'2 (Val.of_bool t2); temp _G p; temp _F q)
     SEP(concrete_mformat G p sigmaG pG; concrete_mformat G' q sigmaG' pG')
-  ). {
-    unfold concrete_mformat.
-    Intros.
-    forward.
-    forward.
-    forward.
-    Exists (first_two_comp && ((Z.of_nat (middle_width G)) <=? (Z.of_nat (middle_width G'))))%bool.
-    entailer!.
-    + rewrite H12. simpl. apply less_components_fact1; auto.
-    + unfold concrete_mformat. entailer!.
-  } {
-    forward.
+  ).
+  { do 3 forward.
+    Exists (first_comp && ((Z.of_nat (middle_width G)) <=? (Z.of_nat (middle_width G'))))%bool.
+    getnw. 
+    unfold concrete_mformat. unnw. subst. entailer!.
+    remember ((Z.of_nat (height G) <=? Z.of_nat (height G')) &&
+    (Z.of_nat (first_line_width G) <=? Z.of_nat (first_line_width G')))%bool as comp eqn:AA.
+    clear AA. subst.
+    simpl. apply less_components_fact1; auto.
+  } 
+  { forward.
     Exists false.
     entailer!.
   }
 
-  Intros first_three_comp.
+  Intros second_comp.
   forward_if(
     EX t3: bool,
-    PROP(t3 = andb first_three_comp
+    PROP(<< third_comp_eq : t3 = andb second_comp
       (((Z.of_nat (last_line_width G))) <=?
-       (Z.of_nat (last_line_width G'))))
+       (Z.of_nat (last_line_width G'))) >>)
     LOCAL(temp _t'3 (Val.of_bool t3); temp _G p; temp _F q)
     SEP(concrete_mformat G p sigmaG pG; concrete_mformat G' q sigmaG' pG')
-  ). {
-    unfold concrete_mformat.
-    Intros.
-    forward.
-    forward.
-    forward.
-    Exists (first_three_comp && (((Z.of_nat (last_line_width G))) <=? (Z.of_nat (last_line_width G'))))%bool.
-    entailer!.
-    + rewrite H13. simpl. apply less_components_fact1; auto.
-    + unfold concrete_mformat. entailer!.
-  } {
+  ). 
+  { do 3 forward.
+    Exists (second_comp && (((Z.of_nat (last_line_width G))) <=? (Z.of_nat (last_line_width G'))))%bool.
+    unfold concrete_mformat. entailer!. simpl.
+    apply less_components_fact1; auto.
+  } 
+  {
     forward.
     Exists false.
     entailer!.
   }
 
-  Intros comparison.
+  Intros third_comp.
   forward.
   Exists (less_components G G').
   entailer!.
-
-  + f_equal. unfold less_components. repeat rewrite less_components_fact2. auto.
-  + unfold concrete_mformat. unfold mformat. Exists sigmaG pG sigmaG' pG'. entailer!.
+  { f_equal. unfold less_components. getnw. subst. repeat rewrite less_components_fact2. auto. }
+  unfold mformat. Exists sigmaG pG sigmaG' pG'. entailer!.
 Qed.
 
 Lemma is_less_than_fact1 x y :
     (x <> y)%nat <-> (x =? y)%nat = false.
 Proof.
-  remember (Nat.eqb_spec x y).
-  clear Heqr.
-  split.
-  - intros. destruct r. contradiction. auto.
-  - intros. destruct r. lia. auto.
+  remember (Nat.eqb_spec x y) eqn:AA. clear AA. split.
+  { intros. destruct r. contradiction. auto. }
+  intros. destruct r. lia. auto.
 Qed.
 
 Lemma is_less_than_fact2 x y
@@ -607,10 +169,10 @@ Lemma is_less_than_fact2 x y
 Proof.
   destruct (Nat.eqb_spec x y).
   { subst. rewrite Int.eq_true. auto. }
-  remember(Int.eq (Int.repr (Z.of_nat x)) (Int.repr (Z.of_nat y))).
+  remember(Int.eq (Int.repr (Z.of_nat x)) (Int.repr (Z.of_nat y))) as b eqn:AA.
   destruct b.
   2: lia.
-  symmetry in Heqb. apply Int.same_if_eq in Heqb. apply repr_inj_unsigned in Heqb; auto. lia.
+  symmetry in AA. apply Int.same_if_eq in AA. apply repr_inj_unsigned in AA; auto. lia.
 Qed.
     
 Lemma body_is_less_than: semax_body Vprog Gprog f_is_less_than is_less_than_spec.
@@ -619,123 +181,138 @@ Proof.
   unfold mformat.
   Intros sigmaG pG sigmaG' pG'.
   forward.
+  getnw. destruct FMT_MP.
   forward_if(
     EX t1: bool,
     PROP(t1 = andb (negb (Nat.eqb (height G) 1%nat)) (Nat.eqb (height G') 1))
     LOCAL(temp _t'2 (Val.of_bool t1); temp _G p; temp _F q)
     SEP(concrete_mformat G p sigmaG pG; concrete_mformat G' q sigmaG' pG')
-  ). {
-    forward.
-    forward.
+  ). 
+  { do 2 forward.
     Exists (negb (height G =? 1)%nat && (height G' =? 1)%nat)%bool.
     entailer!.
-    - f_equal. 
-      assert ((Nat.eqb (height G) 1) = false). destruct (eq_dec (height G) 1%nat).
-      + rewrite e in H11. simpl in H11. list_solve.
-      + apply is_less_than_fact1. auto.
-      + rewrite H21. simpl. apply is_less_than_fact2; auto. simpl. 
-        unfold Int.max_unsigned. simpl. lia.
-    - unfold concrete_mformat. entailer!.
-  } {
-    forward.
+    2: { unfold concrete_mformat. entailer!. unnw. apply mk_format_mp; auto. }
+    f_equal. 
+    assert ((Nat.eqb (height G) 1) = false) as AA. 
+    { destruct (eq_dec (height G) 1%nat).
+      { rewrite e in *. simpl in *. list_solve. }
+      apply is_less_than_fact1. auto. 
+    }
+    rewrite AA. simpl. apply is_less_than_fact2.
+    { getnw. destruct FMT_MP. auto. }
+    unfold Int.max_unsigned; simpl. lia.
+  } 
+  { forward.
     Exists false.
     entailer!.
-    - assert (height G = 1%nat). lia. rewrite H20. simpl. auto.
-    - unfold concrete_mformat. entailer!.
+    2: { unfold concrete_mformat. entailer!. unnw. apply mk_format_mp; auto. }
+    replace (height G) with 1%nat by lia. simpl. auto.
   }
 
+  unfold concrete_mformat.
   Intros first_comp.
+  getnw. destruct FMT_MP.
   forward_if(
     EX t2: bool,
     PROP(t2 = orb first_comp (andb (Nat.eqb (height G) 1%nat) (negb (Nat.eqb (height G') 1%nat))))
     LOCAL(temp _t'3 (Val.of_bool t2); temp _G p; temp _F q)
     SEP(concrete_mformat G p sigmaG pG; concrete_mformat G' q sigmaG' pG')
-  ). {
-    forward.
+  ). 
+  { forward.
     Exists (first_comp || (height G =? 1)%nat && negb (height G' =? 1)%nat)%bool.
     entailer!.
-    rewrite H12. list_solve.
-  } {
-    forward.
+    2: { unfold concrete_mformat. entailer!. unnw. apply mk_format_mp; auto. }
+    remember (negb (height G =? 1)%nat && (height G' =? 1)%nat)%bool as comp eqn:AA.
+    clear AA. subst. 
+    list_solve.
+  } 
+  { forward.
     forward_if(
       EX t3: bool,
       PROP(t3 = andb (Nat.eqb (height G) 1%nat) (negb (Nat.eqb (height G') 1%nat)))
       LOCAL(temp _t'3 (Val.of_bool t3); temp _G p; temp _F q)
       SEP(concrete_mformat G p sigmaG pG; concrete_mformat G' q sigmaG' pG')
-    ). {
-      forward.
-      forward.
-      forward.
+    ). 
+    { do 3 forward.
       Exists ((height G =? 1)%nat && negb (height G' =? 1)%nat)%bool.
       entailer!.
+      2: { unfold concrete_mformat. entailer!. unnw. apply mk_format_mp; auto. }
       - f_equal. replace (height G) with 1%nat by list_solve. simpl. f_equal.
         apply is_less_than_fact2; auto. simpl. unfold Int.max_unsigned. simpl. lia.
-      - unfold concrete_mformat. entailer!.
-    } {
-      forward.
+    } 
+    { forward.
       Exists false.
       entailer!.
+      2: { unfold concrete_mformat. entailer!. unnw. apply mk_format_mp; auto. }
       assert (height G <> 1%nat). list_solve.
       destruct (Nat.eqb_spec (height G) 1%nat).
-      + contradiction.
-      + auto.
-      + unfold concrete_mformat. entailer!.
+      { contradiction. }
+      auto.
     }
     Intros second_comp.
     Exists (first_comp || second_comp)%bool.
     entailer!.
-    rewrite H12.
-    simpl.
-    f_equal.
+    replace (negb (height G =? 1)%nat && (height G' =? 1)%nat)%bool with false.
+    auto.
   }
   Intros all_comp.
-  forward_if. {
-    forward.
+  forward_if. 
+  { forward.
     Exists false.
     unfold is_less_than.
-    destruct (height G).
-    - destruct (height G').
-      + simpl. simpl in H13. lia.
-      + destruct n.
-        * unfold concrete_mformat. unfold mformat. Exists sigmaG pG sigmaG' pG'. entailer!.
-        * simpl in H13. lia.
-    - destruct n.
-      + destruct (height G').
-        * unfold concrete_mformat. unfold mformat. Exists sigmaG pG sigmaG' pG'. entailer!.
-        * destruct n.  
-          { simpl in H13. lia. }
-          { unfold concrete_mformat. unfold mformat. Exists sigmaG pG sigmaG' pG'. entailer!. }
-      + destruct (height G').
-        * simpl in H13. lia.
-        * destruct n0.
-          { unfold concrete_mformat. unfold mformat. Exists sigmaG pG sigmaG' pG'. entailer!. }
-          { simpl in H13. lia. }
+    destruct (height G) eqn:AA.
+    { destruct (height G') eqn:BB.
+      { entailer!. 
+        2: { unfold mformat. Exists sigmaG pG sigmaG' pG'. entailer!. }
+        simpl in *. lia.
+      }
+      entailer!.
+      2: { unfold mformat. Exists sigmaG pG sigmaG' pG'. entailer!. }
+      destruct n.
+      { auto. }
+      simpl in *. lia.
+    }
+    entailer!.
+    2: { unfold mformat. Exists sigmaG pG sigmaG' pG'. entailer!. }
+    destruct n.
+    { destruct (height G').
+      { auto. }
+      destruct n.  
+      2: now auto.
+      simpl in *. lia.
+    }
+    destruct (height G').
+    { simpl in *. lia. }
+    destruct n0.
+    { auto. }
+    simpl in *. lia.
   }
 
   forward_call(p, G, q, G').
-  - unfold concrete_mformat. unfold mformat. Exists sigmaG pG sigmaG' pG'. entailer!.
-  - Intros ans. forward.
-    Exists (less_components G G').
-    entailer!.
-    unfold is_less_than. {
-      destruct (height G).
-      - destruct (height G').
-        + auto.
-        + destruct n.
-          * simpl in H13. lia.
-          * auto.
-      - destruct n.
-        + destruct (height G').
-          * simpl in H13. lia.
-          * destruct n.
-            { auto. }
-            { simpl in H13. lia. }
-        + destruct (height G').
-          * auto.
-          * destruct n0.
-            { simpl in H13. lia. }
-            { auto. }
-    }
+  { unfold mformat. Exists sigmaG pG sigmaG' pG'. entailer!. }
+  Intros ans. forward.
+  Exists (less_components G G').
+  entailer!.
+  unfold is_less_than. 
+  destruct (height G).
+  { destruct (height G').
+    { auto. }
+    destruct n.
+    2: now auto.
+    simpl in *. lia.
+  }
+  destruct n.
+  { destruct (height G').
+    { simpl in *. lia. }
+    destruct n.
+    { auto. }
+    simpl in *. lia.
+  }
+  destruct (height G').
+  { auto. }
+  destruct n0.
+  2: now auto.
+  simpl in *. lia.
 Qed.
 
 Lemma body_empty: semax_body Vprog Gprog f_empty empty_spec.
@@ -743,20 +320,16 @@ Proof.
   start_function.
   forward_call(t_format, gv).
   Intros empty_pointer.
-  destruct (eq_dec empty_pointer nullval). {
-    forward_if(empty_pointer <> nullval).
-    - forward_call. entailer!.
-    - forward. entailer!.
-    - now Intros.
+  destruct (eq_dec empty_pointer nullval).
+  { forward_if(empty_pointer <> nullval).
+    { forward_call. entailer!. }
+    { forward. entailer!. }
+    { now Intros. }
   }
 
-  forward_if(empty_pointer <> nullval). {
-    forward_call.
-    entailer!.
-  } {
-    forward.
-    entailer!.
-  }
+  forward_if(empty_pointer <> nullval). 
+  { forward_call. entailer!. }
+  { forward. entailer!. }
 
   Intros.
   do 6 forward.
@@ -765,9 +338,14 @@ Proof.
   entailer!.
   unfold mformat.
   Exists ([] : (list (Z * list byte))) (Vlong (Int64.repr 0)).
+  unfold concrete_mformat.
   entailer!.
-  - unfold empty. simpl. unfold Int.max_unsigned. simpl. unfold list_mp. repeat (try split; try list_solve; try lia). unfold Int.max_unsigned; simpl; list_solve.
-  - unfold listrep. entailer!.
+  { apply mk_format_mp. 
+    { unfold to_text_eq. auto. }
+    { apply mk_list_mp; auto. simpl. unfold Int.max_unsigned. simpl. lia. }
+    all: now unfold empty.
+  }
+  unfold listrep. entailer!.
 Qed.
 
 Lemma list_byte_to_string_length:
@@ -800,11 +378,11 @@ Proof.
     assert ((Z.to_N (Byte.unsigned a) < 256)%N). {
       list_solve.
     }
-    assert ((N_of_ascii (ascii_of_N (Z.to_N (Byte.unsigned a)))) = Z.to_N (Byte.unsigned a)). {
+    assert ((N_of_ascii (ascii_of_N (Z.to_N (Byte.unsigned a)))) = Z.to_N (Byte.unsigned a)) as AA. {
       apply N_ascii_embedding.
       auto.
     }
-    rewrite H1.
+    rewrite AA.
     rewrite Z2N.id.
     rewrite Byte.repr_unsigned.
     auto.
@@ -826,18 +404,16 @@ Proof.
   start_function.
   forward_call(t_format, gv).
   Intros format_pointer.
-  destruct (eq_dec format_pointer nullval). {
-    forward_if(format_pointer <> nullval).
-    - forward_call. entailer!.
-    - forward. entailer!.
-    - Intros. contradiction.
+  destruct (eq_dec format_pointer nullval). 
+  { forward_if(format_pointer <> nullval).
+    { forward_call. entailer!. }
+    { forward. entailer!. }
+    { Intros. contradiction. }
   }
 
-  forward_if(format_pointer <> nullval). {
-    forward_call. entailer!.
-  } {
-    forward. entailer!.
-  }
+  forward_if(format_pointer <> nullval). 
+  { forward_call. entailer!. } 
+  { forward. entailer!. }
   Intros.
 
   forward.
@@ -850,453 +426,50 @@ Proof.
 
   forward_call(t_list, gv).
   Intros to_text_pointer.
-  destruct (eq_dec to_text_pointer nullval). {
-    forward.
-    forward.
+  destruct (eq_dec to_text_pointer nullval). 
+  { do 2 forward.
     forward_if(to_text_pointer <> nullval).
-    - forward_call. entailer!.
-    - forward. entailer!.
-    - Intros. contradiction.
-  }
-
-  Intros.
-  forward.
-  forward.
-  forward_if(to_text_pointer <> nullval). {
-    forward_call. entailer!.
-  } {
-    forward. entailer.
-  }
-
-  forward.
-  forward.
-  forward.
-  forward.
-  forward.
-  forward.
-  forward.
-  Exists format_pointer.
-  unfold mformat.
-  unfold cstring.
-  Exists ([(0, sigma)]) to_text_pointer.
-  entailer!.
-  - unfold line. simpl. split.
-    + repeat rewrite list_byte_to_string_length. (repeat split; try list_solve; try auto).
-    + unfold to_text_eq. simpl. split.
-      * replace (sigma ++ []) with sigma by list_solve.
-        rewrite empty_string_app.
-        apply list_byte_to_list_byte_eq.
-      * unfold Int.max_unsigned.
-        simpl. unfold list_mp. split. 
-        { unfold Int.max_unsigned. simpl. list_solve. }
-        { 
-          apply Forall_cons.
-          { split. simpl. lia. simpl. auto. }
-          { auto. }
-        }
-  - unfold listrep.
-    Exists (Vlong (Int64.repr 0)) p.
-    unfold cstring.
-    entailer!.
-    unfold line. simpl.
-    repeat rewrite list_byte_to_string_length.
-    entailer!.
-    apply orp_right1.
-    entailer.
-Qed.
-
-
-Lemma list_copy_length_fact:
-  forall (A : Type) (t : list A),
-  Z.to_nat (Zlength t) = Datatypes.length t.
-Proof.
-  intros.
-  induction t.
-  - list_solve.
-  - rewrite Zlength_cons. simpl. 
-    rewrite <- IHt. list_solve.
-Qed.
-
-Lemma singleton_listrep: forall (a : Z) (b : list byte) (h : val) (x: val),
-  cstring Ews b h *
-  malloc_token Ews t_list x *
-  data_at Ews t_list ((Vint (Int.repr a)), (h, nullval)) x
-   |-- listrep [(a, b)] x.
-Proof.
-  intros.
-  unfold listrep.
-  Exists nullval h.
-  entailer!.
-  apply orp_right1.
-  entailer.
-Qed.
-
-Lemma singleton_lseg: forall (a : Z) (b : list byte) (h : val) (x y: val),
-  cstring Ews b h *
-  malloc_token Ews t_list x *
-  data_at Ews t_list ((Vint (Int.repr a)), (h, y)) x
-   |-- lseg [(a, b)] x y.
-Proof.
-  intros.
-  unfold lseg. 
-  Exists y h.
-  entailer!.
-  apply orp_right1.
-  entailer.
-Qed.
-
-Lemma lseg_list: forall (s1 s2: list (Z * list byte)) (x y: val),
-  lseg s1 x y * listrep s2 y |-- listrep (s1 ++ s2) x.
-Proof.
-  induction s1.
-  - intros. simpl. unfold lseg. entailer!.
-  - intros. simpl. unfold lseg; fold lseg. destruct a.
-    Intros h y0.
-    unfold listrep; fold listrep. Exists h y0.
-    entailer!. apply IHs1.
-Qed.
-
-Lemma lseg_lseg: forall (s1 s2: list (Z * list byte)) (x y z: val),
-  lseg s1 x y * lseg s2 y z |-- lseg (s1 ++ s2) x z.
-Proof.
-  intros s1. induction s1.
-  - intros. unfold lseg; fold lseg. simpl. entailer!.
-  - intros. unfold lseg; fold lseg. destruct a. Intros h y0. simpl.
-    unfold lseg; fold lseg.
-    Exists h y0.
-    assert (
-      (emp || malloc_token Ews (Tarray tschar (Zlength l + 1) noattr) y0)
-        * cstring Ews l y0
-        * malloc_token Ews t_list x
-        * data_at Ews t_list (Vint (Int.repr z0), (y0, h)) x
-        * lseg s1 h y
-        * lseg s2 y z
-        |-- 
-      (emp || malloc_token Ews (Tarray tschar (Zlength l + 1) noattr) y0)
-        * cstring Ews l y0
-        * malloc_token Ews t_list x
-        * data_at Ews t_list (Vint (Int.repr z0), (y0, h)) x
-        * (lseg s1 h y
-        * lseg s2 y z)
-    ) as H by entailer!.
-    eapply (derives_trans _ _ _); eauto.
-    apply sepcon_derives; entailer.
-Qed.
-
-Lemma body_list_copy: semax_body Vprog Gprog f_list_copy list_copy_spec.
-Proof.
-  start_function.
-  forward_if(l <> nullval). {
-    forward. Exists nullval. entailer!.
-    destruct H2. assert (nullval = nullval) as Trivial by auto.
-    apply H1 in Trivial as sigma_fact.
-    rewrite sigma_fact.
-    unfold listrep.
-    entailer!.
-  }
-  { forward. entailer!. }
-
-  forward_call(t_list, gv).
-  Intros new_pointer.
-  destruct (eq_dec new_pointer nullval). {
-    forward_if(new_pointer <> nullval).
-    { forward_call. entailer!. }
-    { forward. entailer!. } 
-    { forward. contradiction. }
-  }
-
-  forward_if(new_pointer <> nullval).
-  { forward_call. entailer!. }
-  { forward. entailer!. }
-
-  Intros. do 2 forward.
-  
-  forward_loop (
-    EX i : Z, EX cur : val, EX l_cur : val,
-    PROP(0 <= i < Zlength sigma + 1;
-         cur <> nullval;
-         l_cur <> nullval)
-    LOCAL(temp _new new_pointer; 
-          temp _l l;
-          temp _cur cur; 
-          temp _l_cur l_cur; 
-          gvars gv)
-    SEP(malloc_token Ews t_list cur;
-        data_at_ Ews t_list cur;
-        lseg (sublist 0 i sigma) new_pointer cur; 
-        lseg (sublist 0 i sigma) l l_cur;
-        listrep (sublist i (Zlength sigma) sigma) l_cur;
-        mem_mgr gv)
-  ) break: (
-    PROP()
-    LOCAL(temp _new new_pointer; gvars gv)
-    SEP(listrep sigma new_pointer; listrep sigma l; mem_mgr gv)
-  ).
-  3: { forward. Exists new_pointer. entailer!. }
-  {
-    Exists 0 new_pointer l.
-    entailer!.
-    replace (sublist 0 0 sigma) with ([] : list (Z * list byte)) by list_solve.
-    unfold lseg.
-    replace (sublist 0 (Zlength sigma) sigma) with sigma by list_solve.
-    entailer!.
-  }
-  
-  Intros i cur l_cur.
-  rename H2 into I_Boundaries.
-  rename H1 into L_not_null.
-  rename n into New_pointer_not_null.
-  rename H3 into Cur_not_null.
-  rename H4 into L_cur_not_null.
-  destruct (eq_dec i (Zlength sigma)) as [ | I_is_not_zlength]. {
-    subst.
-    replace ((sublist (Zlength sigma) (Zlength sigma) sigma)) with ([] : list (Z * list byte)) by list_solve.
-    unfold listrep; fold listrep. 
-    Intros. contradiction.
-  }
-
-replace (sublist i (Zlength sigma) sigma) with 
-  (Znth i sigma :: sublist (i + 1) (Zlength sigma) sigma) by list_solve.
-unfold listrep; fold listrep.
-remember (Znth i sigma) as ith_element.
-destruct ith_element as (shift_i, line_i).
-
-Intros l_cur_tail line_i_pointer.
-do 3 forward.
-forward_call(Ews, line_i, line_i_pointer).
-forward_call((Tarray tschar (Zlength line_i + 1) noattr), gv). {
-  assert (In (shift_i, line_i) sigma) as In_fact. 
-  { rewrite Heqith_element. apply Znth_In. lia. }
-
-  assert (Zlength line_i + 1 <= Int.max_unsigned) as Zlength_fact. {
-    remember (fun x : Z * list byte =>
-    0 <= fst x <= Int.max_unsigned /\
-    0 <= Zlength (snd x) + 1 <= Int.max_unsigned) as List_condition.
-    assert (List_condition (shift_i, line_i)) as Ith_condition. 
-    { apply (computable_theorems.Forall_forall1 _ sigma); auto. }
-    rewrite HeqList_condition in Ith_condition.
-    destruct Ith_condition as [shift_condition].
-    simpl in H1. lia.
-  }
-
-  unfold sizeof. unfold Ctypes.sizeof.
-  unfold Int.max_unsigned in Zlength_fact. simpl in Zlength_fact.
-  unfold Ptrofs.max_unsigned. simpl.
-  lia.
-}
-
-Intros cur_line_i_pointer.
-destruct (eq_dec cur_line_i_pointer nullval). {
-  do 2 forward.
-  forward_if(cur_line_i_pointer <> nullval).
-  { forward_call. entailer!. }
-  { forward. entailer!. }
-  { forward. contradiction. }
-}
-
-Intros. do 2 forward.
-forward_if(cur_line_i_pointer <> nullval).
-{ forward_call. entailer!. }
-{ forward. entailer!. }
-
-do 2 forward.
-forward_call(Ews, Ews, cur_line_i_pointer, Zlength line_i + 1, line_i_pointer, line_i).
-do 2 forward.
-
-forward_if(l_cur_tail <> nullval). {
-  do 2 forward.
-  entailer!.
-  rewrite <- cstringn_equiv.
-  assert (i + 1 = Zlength sigma) as AA. {
-    assert (i + 1 < Zlength sigma \/ i + 1 = Zlength sigma) as BB. lia.
-    destruct BB. {
-      replace (sublist (i + 1) (Zlength sigma) sigma) 
-        with (Znth (i + 1) sigma :: (sublist (i + 2) (Zlength sigma) sigma)) in H12 by list_solve.
-        destruct H12.
-      assert( Znth (i + 1) sigma :: sublist (i + 2) (Zlength sigma) sigma = []) as CC by auto.
-      inversion CC.
-    }
-    auto.
-  }
-  rewrite AA.
-  replace (sublist (Zlength sigma) (Zlength sigma) sigma) with ([] : list (Z * list byte)) by list_solve.
-  unfold listrep; fold listrep.
-  
-  entailer!.
-
-  assert (
-    cstring Ews line_i cur_line_i_pointer 
-      * cstring Ews line_i line_i_pointer
-      * malloc_token Ews (Tarray tschar (Zlength line_i + 1) noattr) cur_line_i_pointer
-      * malloc_token Ews t_list cur
-      * data_at Ews t_list (Vint (Int.repr shift_i), (cur_line_i_pointer, Vlong (Int64.repr 0))) cur
-      * lseg (sublist 0 i sigma) new_pointer cur
-      * lseg (sublist 0 i sigma) l l_cur
-      * (emp || malloc_token Ews (Tarray tschar (Zlength line_i + 1) noattr) line_i_pointer)
-      * malloc_token Ews t_list l_cur
-      * data_at Ews t_list (Vint (Int.repr shift_i), (line_i_pointer, nullval)) l_cur
-    |-- 
-    (lseg (sublist 0 i sigma) new_pointer cur *
-    (
-      malloc_token Ews (Tarray tschar (Zlength line_i + 1) noattr) cur_line_i_pointer
-      * cstring Ews line_i cur_line_i_pointer 
-      * malloc_token Ews t_list cur
-      * data_at Ews t_list (Vint (Int.repr shift_i), (cur_line_i_pointer, Vlong (Int64.repr 0))) cur
-    )) * (
-      lseg (sublist 0 i sigma) l l_cur *
-      (
-      (emp || malloc_token Ews (Tarray tschar (Zlength line_i + 1) noattr) line_i_pointer)
-      * cstring Ews line_i line_i_pointer
-      * malloc_token Ews t_list l_cur
-      * data_at Ews t_list (Vint (Int.repr shift_i), (line_i_pointer, nullval)) l_cur
-      )
-    )
-  ) as Trans_step1. 
-  { entailer!. }
-
-  eapply (derives_trans _ _ _); eauto. 
-  apply sepcon_derives. 
-  {
-    assert (sigma = sublist 0 i sigma ++ sublist i (Zlength sigma) sigma) as FF by list_solve.
-    rewrite FF.
-    assert (
-      lseg (sublist 0 i (sublist 0 i sigma ++ sublist i (Zlength sigma) sigma)) new_pointer cur
-       * (malloc_token Ews (Tarray tschar (Zlength line_i + 1) noattr) cur_line_i_pointer
-       * cstring Ews line_i cur_line_i_pointer
-       * malloc_token Ews t_list cur
-       * data_at Ews t_list (Vint (Int.repr shift_i), (cur_line_i_pointer, Vlong (Int64.repr 0))) cur)
-       |-- 
-      lseg (sublist 0 i (sublist 0 i sigma ++ sublist i (Zlength sigma) sigma)) new_pointer cur *
-      listrep [(shift_i, line_i)] cur
-    ) as Trans_step2. {
-      unfold listrep; fold listrep.
-      Exists nullval cur_line_i_pointer.
-      entailer!. apply orp_right2. entailer.
-    }
-
-    eapply (derives_trans _ _ _); eauto.
-    rewrite Heqith_element.
-    replace [Znth i sigma] with (sublist i (Zlength sigma) sigma) by list_solve.
-    replace (sublist 0 i sigma ++ sublist i (Zlength sigma) sigma) with sigma at 1 by list_solve.
-    apply lseg_list.
-  }
-  {
-    assert (sigma = sublist 0 i sigma ++ sublist i (Zlength sigma) sigma) as FF by list_solve.
-    rewrite FF.
-    assert (
-      lseg (sublist 0 i (sublist 0 i sigma ++ sublist i (Zlength sigma) sigma)) l l_cur
-        * ((emp || malloc_token Ews (Tarray tschar (Zlength line_i + 1) noattr) line_i_pointer)
-          * cstring Ews line_i line_i_pointer
-          * malloc_token Ews t_list l_cur
-          * data_at Ews t_list (Vint (Int.repr shift_i), (line_i_pointer, nullval)) l_cur)
-      |-- 
-      lseg (sublist 0 i (sublist 0 i sigma ++ sublist i (Zlength sigma) sigma)) l l_cur *
-      listrep [(shift_i, line_i)] l_cur
-    ) as Trans_step2. {
-      unfold listrep; fold listrep.
-      Exists nullval line_i_pointer.
-      entailer!.
-    }
-
-    eapply (derives_trans _ _ _); eauto.
-    rewrite Heqith_element.
-    replace [Znth i sigma] with (sublist i (Zlength sigma) sigma) by list_solve.
-    replace (sublist 0 i sigma ++ sublist i (Zlength sigma) sigma) with sigma at 1 by list_solve.
-    apply lseg_list.
-  }
-  }
-  { forward. entailer!. }
-  Intros.
-  forward_call(t_list, gv).
-  Intros cur_tail.
-  do 2 forward.
-  destruct (eq_dec cur_tail nullval). {
-    forward_if(cur_tail <> nullval).
     { forward_call. entailer!. }
     { forward. entailer!. }
-    { forward. contradiction. }
+    { Intros. contradiction. }
   }
-  forward_if(cur_tail <> nullval). 
-  { forward_call. entailer!. }
-  { forward. entailer!. }
+
   Intros.
-
   do 2 forward.
-  Exists (i + 1) cur_tail l_cur_tail.
-  entailer!.
-  rewrite <- cstringn_equiv.
+  forward_if(to_text_pointer <> nullval). 
+  { forward_call. entailer!. } 
+  { forward. entailer. }
 
-  assert (
-    cstring Ews line_i cur_line_i_pointer * cstring Ews line_i line_i_pointer
-    * malloc_token Ews (Tarray tschar (Zlength line_i + 1) noattr) cur_line_i_pointer
-    * malloc_token Ews t_list cur
-    * data_at Ews t_list (Vint (Int.repr shift_i), (cur_line_i_pointer, cur_tail)) cur
-    * lseg (sublist 0 i sigma) new_pointer cur
-    * lseg (sublist 0 i sigma) l l_cur
-    * (emp || malloc_token Ews (Tarray tschar (Zlength line_i + 1) noattr) line_i_pointer)
-    * malloc_token Ews t_list l_cur
-    * data_at Ews t_list (Vint (Int.repr shift_i), (line_i_pointer, l_cur_tail)) l_cur
-    |--
-    (lseg (sublist 0 i sigma) new_pointer cur
-    * (malloc_token Ews (Tarray tschar (Zlength line_i + 1) noattr) cur_line_i_pointer
-    * cstring Ews line_i cur_line_i_pointer
-    * malloc_token Ews t_list cur
-    * data_at Ews t_list (Vint (Int.repr shift_i), (cur_line_i_pointer, cur_tail)) cur))
-    * (lseg (sublist 0 i sigma) l l_cur
-    * ((emp || malloc_token Ews (Tarray tschar (Zlength line_i + 1) noattr) line_i_pointer)
-    * cstring Ews line_i line_i_pointer
-    * malloc_token Ews t_list l_cur
-    * data_at Ews t_list (Vint (Int.repr shift_i), (line_i_pointer, l_cur_tail)) l_cur))
-  ) as AA by entailer!.
-  
-  eapply (derives_trans _ _ _); eauto.
-  apply sepcon_derives. {
-    clear AA.
-    assert (
-      lseg (sublist 0 i sigma) new_pointer cur
-       * (malloc_token Ews (Tarray tschar (Zlength line_i + 1) noattr) cur_line_i_pointer
-       * cstring Ews line_i cur_line_i_pointer
-       * malloc_token Ews t_list cur
-       * data_at Ews t_list (Vint (Int.repr shift_i), (cur_line_i_pointer, cur_tail)) cur)
-      |-- 
-      lseg (sublist 0 i sigma) new_pointer cur * 
-      lseg (sublist i (i + 1) sigma) cur cur_tail
-    ). {
-      apply sepcon_derives. entailer.
-      replace (sublist i (i + 1) sigma) with [Znth i sigma] by list_solve.
-      unfold lseg.
-      rewrite <- Heqith_element.
-      Exists cur_tail cur_line_i_pointer.
-      entailer!.
-      apply orp_right2. entailer.
+  do 7 forward.
+  Exists format_pointer.
+  unfold mformat. unfold cstring.
+  Exists ([(0, sigma)]) to_text_pointer.
+  entailer!. unfold concrete_mformat.
+  entailer!.
+  { 
+    unnw. apply mk_format_mp.
+    { unfold to_text_eq. unfold to_text. simpl.
+      replace (sigma ++ []) with sigma by list_solve.
+      rewrite empty_string_app.
+      apply list_byte_to_list_byte_eq.
     }
-    eapply (derives_trans _ _ _); eauto.
-    replace (sublist 0 (i + 1) sigma) with (sublist 0 i sigma ++ sublist i (i + 1) sigma) by list_solve.
-    apply lseg_lseg.
-  }
-  {
-    clear AA.
-    assert (
-      lseg (sublist 0 i sigma) l l_cur
-      * ((emp || malloc_token Ews (Tarray tschar (Zlength line_i + 1) noattr) line_i_pointer)
-      * cstring Ews line_i line_i_pointer
-      * malloc_token Ews t_list l_cur
-      * data_at Ews t_list (Vint (Int.repr shift_i), (line_i_pointer, l_cur_tail)) l_cur)
-      |-- 
-      lseg (sublist 0 i sigma) l l_cur * 
-      lseg (sublist i (i + 1) sigma) l_cur l_cur_tail
-    ). {
-      apply sepcon_derives. entailer.
-      replace (sublist i (i + 1) sigma) with [Znth i sigma] by list_solve.
-      unfold lseg.
-      rewrite <- Heqith_element.
-      Exists l_cur_tail line_i_pointer.
-      entailer!.
+    { apply mk_list_mp; auto.
+      { simpl. unfold Int.max_unsigned. simpl. lia. }
+      list_simplify. simpl. lia.
     }
-    eapply (derives_trans _ _ _); eauto.
-    replace (sublist 0 (i + 1) sigma) with (sublist 0 i sigma ++ sublist i (i + 1) sigma) by list_solve.
-    apply lseg_lseg.
+    all: unfold line; simpl.
+    { unfold Int.max_unsigned. simpl. lia. }
+    all: rewrite list_byte_to_string_length; list_solve.
   }
+  unfold listrep.
+  unfold cstring.
+  Exists (Vlong (Int64.repr 0)) p.
+  entailer!.
+  unfold line; simpl.
+  repeat rewrite list_byte_to_string_length.
+  entailer!.
+  apply orp_right1.
+  entailer.
 Qed.
 
 Lemma sp_fact1 (n : Z):
