proof/format_specs.v
@@ -1,0 +1,284 @@
+Require Import HahnBase.
+
+Require Import VST.floyd.proofauto.
+Require Import VST.floyd.library.
+Require Import printer.printer_files.compiled_format.
+Require Import printer.verified_printer.Format.
+Require Import Coq.Strings.Ascii.
+
+Instance CompSpecs : compspecs. make_compspecs prog. Defined.
+Definition Vprog : varspecs. mk_varspecs prog. Defined.
+
+Definition t_list := Tstruct _list noattr.
+Definition t_format := Tstruct _t noattr.
+
+Definition max_spec : ident * funspec := 
+DECLARE _max
+  WITH a : Z, b : Z
+  PRE [ tuint, tuint ]
+    PROP (
+      0 <= a <= Int.max_unsigned;
+      0 <= b <= Int.max_unsigned
+    )
+    PARAMS (Vint (Int.repr a); Vint (Int.repr b))
+    SEP ()
+  POST [ tuint ] EX q : Z,
+    PROP (q = Z.max a b) 
+    RETURN (Vint (Int.repr q)) 
+    SEP().
+
+Definition strlen_spec :=
+ DECLARE _strlen
+  WITH sh: share, s : list byte, str: val
+  PRE [ tptr tschar ]
+    PROP (readable_share sh)
+    PARAMS (str)
+    SEP (cstring sh s str)
+  POST [ size_t ]
+    PROP ()
+    RETURN (Vptrofs (Ptrofs.repr (Zlength s)))
+    SEP (cstring sh s str).
+
+Definition strcpy_spec :=
+ DECLARE _strcpy
+  WITH wsh: share, rsh: share, dest : val, n : Z, src : val, s : list byte
+  PRE [ tptr tschar, tptr tschar ]
+    PROP (writable_share wsh; readable_share rsh; Zlength s < n)
+    PARAMS (dest; src)
+    SEP (data_at_ wsh (tarray tschar n) dest; cstring rsh s src)
+  POST [ tptr tschar ]
+    PROP ()
+    RETURN (dest)
+    SEP (cstringn wsh s n dest; cstring rsh s src).
+
+Definition strcat_spec :=
+ DECLARE _strcat
+  WITH wsh: share, rsh: share, dest : val, n : Z, src : val, b : list byte, s : list byte
+  PRE [ tptr tschar, tptr tschar ]
+    PROP (writable_share wsh; readable_share rsh; Zlength b + Zlength s < n)
+    PARAMS (dest; src)
+    SEP (cstringn wsh b n dest; cstring rsh s src)
+  POST [ tptr tschar]
+    PROP ()
+    RETURN (dest)
+    SEP (cstringn wsh (b ++ s) n dest; cstring rsh s src).
+
+Fixpoint listrep (sigma: list (Z * (list byte))) (p: val) : mpred :=
+ match sigma with
+ | (a, b)::hs =>
+    EX x:val, EX y: val,
+    (emp || malloc_token Ews (Tarray tschar (Zlength b + 1) noattr) y) *
+    cstring Ews b y *
+    malloc_token Ews t_list p * 
+    data_at Ews t_list ((Vint (Int.repr a), (y, x)) : @reptype CompSpecs t_list) p *
+    listrep hs x
+ | nil =>
+    !! (<< LIST_NULL_PTR : p = nullval >> ) && emp
+ end.
+
+Arguments listrep sigma p : simpl never.
+
+Lemma listrep_local_facts:
+  forall sigma p,
+   listrep sigma p |--
+   !! (<< LIST_PTR_FACT : is_pointer_or_null p /\ (p=nullval <-> sigma=nil) >>).
+Proof.
+  intros.
+
+  revert p; induction sigma; intros p.
+  { unfold listrep. unnw. entailer!. split; auto. }
+  unfold listrep; fold listrep. destruct a. entailer. unnw. entailer!. split; intro.
+  2: now auto.
+  subst. eapply field_compatible_nullval; eauto.
+Qed.
+#[export] Hint Resolve listrep_local_facts : saturate_local.
+
+Lemma listrep_valid_pointer:
+  forall sigma p,
+   listrep sigma p |-- valid_pointer p.
+Proof.
+  intros.
+  unfold listrep. destruct sigma; simpl; unnw.
+  { entailer!. }
+  destruct p0. Intros x y. auto with valid_pointer.
+Qed.
+#[export] Hint Resolve listrep_valid_pointer : valid_pointer.
+
+Fixpoint lseg (sigma: list (Z * (list byte))) (x z: val) : mpred :=
+  match sigma with
+  | nil => !! (<< LSEG_PTR_FACT : x = z >>) && emp
+  | (a, b)::hs => EX h: val, EX y:val, 
+        (emp || malloc_token Ews (Tarray tschar (Zlength b + 1) noattr) y) *
+        cstring Ews b y *
+        malloc_token Ews t_list x * 
+        data_at Ews t_list ((Vint (Int.repr a)), (y, h)) x * 
+        lseg hs h z
+  end.
+
+Arguments lseg sigma x z : simpl never.
+
+Definition list_copy_spec : ident * funspec :=
+DECLARE _list_copy
+  WITH sh : share, l : val, sigma : list (Z * (list byte)), gv: globals
+  PRE [ tptr t_list ]
+    PROP(0 <= Zlength sigma <= Int.max_unsigned;
+         Forall (fun x => 0 <= (fst x) <= Int.max_unsigned /\ 0 <= Zlength (snd x) + 1 <= Int.max_unsigned) sigma)
+    PARAMS(l) GLOBALS(gv)
+    SEP(listrep sigma l; mem_mgr gv)
+  POST [ tptr t_list ] 
+    EX q: val,
+    PROP()
+    RETURN(q)
+    SEP(listrep sigma l; listrep sigma q; mem_mgr gv).
+
+
+Fixpoint string_to_list_byte (s: string) : list byte :=
+  match s with
+  | EmptyString => nil
+  | String a s' => Byte.repr (Z.of_N (Ascii.N_of_ascii a))
+                                      :: string_to_list_byte s'
+  end.
+
+Fixpoint text_from (sigma : list (Z * list byte)) : list byte :=
+  match sigma with 
+  | nil => nil
+  | (s, l)::hs => (repeat (Byte.repr (Z.of_N 32)) (Z.to_nat s) ) ++ l ++ text_from hs
+end.
+
+Definition to_text_eq (to_text : nat -> string -> string) (sigma : list (Z * list byte)) :=
+  string_to_list_byte (to_text (Z.to_nat 0) EmptyString) = text_from sigma.
+
+Record list_mp (sigma : list (Z * list byte)) : Prop :=
+  mk_list_mp {
+    list_mp_length     : 0 <= Zlength sigma + 1 <= Int.max_unsigned;
+    list_mp_forall_fst :
+      Forall (fun x => 0 <= (fst x) <= Int.max_unsigned) sigma;
+    list_mp_forall_snd :
+      Forall (fun x => 0 <= Zlength (snd x) + 1 <= Int.max_unsigned) sigma;
+  }.
+
+Record format_mp (G : t) (sigma : list (Z * list byte)) : Prop :=
+  mk_format_mp {
+    format_mp_text_eq : to_text_eq G.(to_text) sigma;
+    format_mp_list_mp : list_mp sigma;
+    format_mp_hg : 0 <= Z.of_nat (height G) <= Int.max_unsigned;
+    format_mp_flw : 0 <= Z.of_nat (first_line_width G) <= Int.max_unsigned;
+    format_mp_mw : 0 <= Z.of_nat (middle_width G) <= Int.max_unsigned;
+    format_mp_llw : 0 <= Z.of_nat (last_line_width G) <= Int.max_unsigned;
+  }.
+
+ Definition concrete_mformat (G : t) (x : val) (sigma : list (Z * list byte)) (p : val) : mpred :=
+  !! (<< FMT_MP : format_mp G sigma >> ) &&
+  sepcon (malloc_token Ews t_format x)
+  (sepcon 
+  (data_at Ews t_format (Vint (Int.repr (Z.of_nat G.(height))),
+                        (Vint (Int.repr (Z.of_nat G.(first_line_width))),
+                         (Vint (Int.repr (Z.of_nat G.(middle_width))),
+                          (Vint (Int.repr (Z.of_nat G.(last_line_width))), p)))) x)
+  (listrep sigma p))
+.
+
+Definition mformat (G : t) (x : val) : mpred := 
+  EX sigma : list (Z * list byte), 
+  EX p : val,
+  concrete_mformat G x sigma p
+ .
+
+ Definition less_components_spec : ident * funspec :=
+ DECLARE _less_components
+  WITH p : val, G : t, q : val, G' : t
+  PRE [ tptr t_format, tptr t_format]
+    PROP()
+    PARAMS(p; q)
+    SEP(mformat G p; mformat G' q)
+  POST [ tbool ]
+    EX a : bool,
+    PROP(a = less_components G G')
+    RETURN(Val.of_bool a)
+    SEP(mformat G p; mformat G' q).
+
+
+Definition is_less_than_spec : ident * funspec :=
+DECLARE _is_less_than
+  WITH p : val, G : t, q : val, G' : t
+  PRE [ tptr t_format, tptr t_format]
+    PROP()
+    PARAMS(p; q)
+    SEP(mformat G p; mformat G' q)
+  POST [ tbool ]
+    EX a : bool,
+    PROP(a = is_less_than G G')
+    RETURN(Val.of_bool a)
+    SEP(mformat G p; mformat G' q).
+
+
+Definition empty_spec : ident * funspec :=
+DECLARE _empty 
+  WITH gv : globals
+  PRE []
+    PROP()
+    PARAMS() GLOBALS(gv)
+    SEP(mem_mgr gv)
+  POST [ tptr t_format ]
+    EX p : val,
+    PROP()
+    RETURN(p)
+    SEP(mem_mgr gv; mformat empty p).
+
+
+Fixpoint list_byte_to_string (sigma: list byte) : string :=
+  match sigma with 
+  | nil => EmptyString
+  | (h :: hs) => String (Ascii.ascii_of_N (Z.to_N (Byte.unsigned h))) (list_byte_to_string hs)
+  end.
+
+
+Definition line_spec : ident * funspec :=
+DECLARE _line
+  WITH p : val, sigma : list byte, gv : globals
+  PRE [ tptr tschar ]
+    PROP(0 <= Zlength sigma + 1 <= Int.max_unsigned)
+    PARAMS(p) GLOBALS(gv)
+    SEP(mem_mgr gv; cstring Ews sigma p)
+  POST [ tptr t_format ]
+    EX q : val,
+    PROP()
+    RETURN(q)
+    SEP(mem_mgr gv; mformat (line (list_byte_to_string sigma)) q).
+    
+
+Definition sp_spec : ident * funspec :=
+DECLARE _sp
+  WITH n : Z, gv : globals
+  PRE [ size_t ]
+    PROP (0 <= n <= Int.max_unsigned)
+    PARAMS(Vptrofs (Ptrofs.repr n)) GLOBALS(gv)
+    SEP(mem_mgr gv)
+  POST [ tptr tschar ]
+    EX p : val,
+    PROP()
+    RETURN(p)
+    SEP(cstring Ews (string_to_list_byte (sp (Z.to_nat n))) p;
+         malloc_token Ews (Tarray tschar (n + 1) noattr) p; mem_mgr gv).
+
+Definition add_above_spec : ident * funspec :=
+DECLARE _add_above
+  WITH G : t, F : t, pointer_G : val, pointer_F : val, gv : globals
+  PRE [ tptr t_format, tptr t_format ]
+    PROP ()
+    PARAMS(pointer_G; pointer_F) GLOBALS(gv)
+    SEP(mformat G pointer_G; mformat F pointer_F; mem_mgr gv)
+  POST [ tptr t_format ]
+    EX p : val,
+    PROP()
+    RETURN(p)
+    SEP(mformat G pointer_G; mformat F pointer_F; 
+        mformat (add_above G F) p; mem_mgr gv).
+
+
+Definition Gprog : funspecs :=
+        ltac:(with_library prog [
+                   max_spec; strlen_spec; strcpy_spec; strcat_spec;
+                   list_copy_spec; less_components_spec; is_less_than_spec; 
+                   empty_spec; line_spec; sp_spec
+ ]).
