proof/format_std_proof.v
@@ -1,0 +1,537 @@
+Require Import HahnBase.
+
+Require Import VST.floyd.proofauto.
+Require Import VST.floyd.library.
+Require Import printer.printer_files.compiled_format.
+Require Import printer.verified_printer.Format.
+Require Import Coq.Strings.Ascii.
+Require Import format_specs.
+
+Lemma body_max: semax_body Vprog Gprog f_max max_spec.
+Proof.
+  start_function. 
+  forward_if.
+  { forward. Exists b. entailer!. }
+  forward. Exists a. entailer!.
+Qed.
+
+Lemma body_strlen: semax_body Vprog Gprog f_strlen strlen_spec.
+Proof.
+  start_function.
+  unfold cstring in *.
+  Intros.
+  forward.
+
+  forward_loop  (EX i : Z,
+    PROP (0 <= i < Zlength s + 1)
+    LOCAL (temp _str str; temp _i (Vptrofs (Ptrofs.repr i)))
+    SEP (data_at sh (tarray tschar (Zlength s + 1))
+            (map Vbyte (s ++ [Byte.zero])) str)).
+
+  { Exists 0. entailer. }
+  Intros i. forward. forward_if. forward. entailer!. 
+  repeat f_equal. cstring.
+  forward. entailer. Exists (i + 1). entailer!.
+  assert(0 <= i + 1 < Zlength (s ++ [Byte.zero])) as AA.
+  { assert (i < Zlength s) by cstring.
+    autorewrite with sublist.
+    cstring. }
+  autorewrite with sublist in AA. simpl in AA.
+  apply AA.
+Qed.
+
+Lemma body_strcpy : semax_body Vprog Gprog f_strcpy strcpy_spec.
+Proof.
+  start_function.
+
+  unfold cstring,cstringn in *.
+  forward.
+
+  forward_loop (EX i : Z,
+    PROP (0 <= i < Zlength s + 1)
+    LOCAL (temp _i (Vptrofs (Ptrofs.repr i)); temp _dest dest; temp _src src)
+    SEP (data_at wsh (tarray tschar n)
+          (map Vbyte (sublist 0 i s) ++ Zrepeat Vundef (n - i)) dest;
+         data_at rsh (tarray tschar (Zlength s + 1)) (map Vbyte (s ++ [Byte.zero])) src)).
+  { Exists 0. entailer. }
+  Intros i. forward. forward. forward. forward_if.
+  { forward. entailer!. apply derives_refl'. f_equal.
+    rewrite upd_Znth_app2.
+    2: { list_solve. }
+    assert (i - Zlength (map Vbyte (sublist 0 i s)) = 0) as AA by list_solve.
+    rewrite AA. unfold Zrepeat.
+    remember (Z.to_nat (n - i)). destruct n0.
+    { lia. }
+    simpl. 
+    assert (i = Zlength s) by cstring.
+    replace (Z.to_nat (n - (Zlength s + 1))) with n0 by lia.
+    list_solve. }
+  forward. Exists (i + 1). entailer!. 
+  2: { rewrite upd_Znth_app2.
+       all: list_solve. }
+  assert (0 <= i + 1 < (Zlength (s ++ [Byte.zero]))) as AA.
+  { assert (i < Zlength s) as LT by cstring.
+    autorewrite with sublist.
+    cstring. }
+  autorewrite with sublist in AA. simpl in AA.
+  apply AA.
+Qed.
+
+Lemma body_strcat: semax_body Vprog Gprog f_strcat strcat_spec.
+Proof.
+  leaf_function.
+  start_function.
+  unfold cstringn, cstring in *.
+  forward.
+  forward_loop(
+    EX i : Z,
+    PROP (0 <= i < Zlength b + 1)
+    LOCAL (temp _i (Vptrofs (Ptrofs.repr i)); temp _dest dest; temp _src src)
+    SEP (cstringn wsh b n dest; cstring rsh s src))
+  break:
+  (
+    PROP ()
+    LOCAL (temp _i (Vptrofs (Ptrofs.repr (Zlength b))); temp _dest dest; temp _src src)
+    SEP (cstringn wsh b n dest; cstring rsh s src)).
+  { Exists 0. unfold cstringn, cstring. entailer!. }
+  { unfold cstringn, cstring.
+    Intros i.
+    forward. 
+    { entailer!. }
+    { entailer!. list_solve. }
+    autorewrite with sublist norm.
+    forward.
+    forward_if.
+    { forward. unfold cstringn, cstring. entailer!. do 2 f_equal. list_solve. }
+    forward.
+    Exists (i + 1).
+    unfold cstringn, cstring.
+    entailer!.
+    list_solve.
+  }
+  unfold cstringn, cstring.
+  forward.
+  autorewrite with sublist norm in *.
+  forward_loop(
+    EX j : Z,
+    PROP (0 <= j < Zlength s + 1)
+    LOCAL (temp _i (Vptrofs (Ptrofs.repr (Zlength b)));
+            temp _j (Vptrofs (Ptrofs.repr j));
+            temp _dest dest; temp _src src)
+    SEP ( data_at wsh (tarray tschar n) (map Vbyte (b ++ sublist 0 j s) ++ 
+    Zrepeat Vundef (n - (Zlength b + j))) dest;
+        cstring rsh s src)
+  ).
+  { Exists 0. unfold cstring, cstringn. autorewrite with sublist norm. entailer!. list_solve. }
+  Intros j.
+  unfold cstringn, cstring.
+  autorewrite with sublist norm in *.
+  Intros.
+  do 3 forward.
+  { entailer!. }
+  forward_if.
+  { forward. autorewrite with sublist norm. entailer!; list_solve. }
+  forward.
+  Exists (j + 1).
+  entailer!.
+  { list_solve. }
+  unfold cstringn, cstring.
+  autorewrite with sublist norm.
+  entailer!.
+  list_solve.
+Qed.
+
+Lemma list_copy_length_fact:
+  forall (A : Type) (t : list A),
+  Z.to_nat (Zlength t) = Datatypes.length t.
+Proof.
+  intros.
+  induction t.
+  { list_solve. }
+  rewrite Zlength_cons. simpl. 
+  rewrite <- IHt. list_solve.
+Qed.
+
+Lemma singleton_listrep: forall (a : Z) (b : list byte) (h : val) (x: val),
+  cstring Ews b h *
+  malloc_token Ews t_list x *
+  data_at Ews t_list ((Vint (Int.repr a)), (h, nullval)) x
+   |-- listrep [(a, b)] x.
+Proof.
+  intros.
+  unfold listrep.
+  Exists nullval h.
+  entailer!.
+  apply orp_right1.
+  entailer.
+Qed.
+
+Lemma singleton_lseg: forall (a : Z) (b : list byte) (h : val) (x y: val),
+  cstring Ews b h *
+  malloc_token Ews t_list x *
+  data_at Ews t_list ((Vint (Int.repr a)), (h, y)) x
+   |-- lseg [(a, b)] x y.
+Proof.
+  intros.
+  unfold lseg. 
+  Exists y h.
+  entailer!.
+  apply orp_right1.
+  entailer.
+Qed.
+
+Lemma lseg_list: forall (s1 s2: list (Z * list byte)) (x y: val),
+  lseg s1 x y * listrep s2 y |-- listrep (s1 ++ s2) x.
+Proof.
+  induction s1.
+  { intros. simpl. unfold lseg. entailer!. unnw. subst. entailer. }
+  intros. simpl. unfold lseg; fold lseg. destruct a.
+  Intros h y0.
+  unfold listrep; fold listrep. Exists h y0.
+  entailer!. apply IHs1.
+Qed.
+
+Lemma lseg_lseg: forall (s1 s2: list (Z * list byte)) (x y z: val),
+  lseg s1 x y * lseg s2 y z |-- lseg (s1 ++ s2) x z.
+Proof.
+  intros s1. induction s1.
+  { intros. unfold lseg; fold lseg. simpl. entailer!. unnw. subst. entailer. }
+  intros. unfold lseg; fold lseg. destruct a. Intros h y0. simpl.
+  unfold lseg; fold lseg.
+  Exists h y0.
+  assert (
+    (emp || malloc_token Ews (Tarray tschar (Zlength l + 1) noattr) y0)
+      * cstring Ews l y0
+      * malloc_token Ews t_list x
+      * data_at Ews t_list (Vint (Int.repr z0), (y0, h)) x
+      * lseg s1 h y
+      * lseg s2 y z
+      |-- 
+    (emp || malloc_token Ews (Tarray tschar (Zlength l + 1) noattr) y0)
+      * cstring Ews l y0
+      * malloc_token Ews t_list x
+      * data_at Ews t_list (Vint (Int.repr z0), (y0, h)) x
+      * (lseg s1 h y
+      * lseg s2 y z)
+  ) as H by entailer!.
+  eapply (derives_trans _ _ _); eauto.
+  apply sepcon_derives; entailer.
+Qed.
+
+Definition list_copy_loop_invariant 
+(l new_pointer : val)
+(sigma : list (Z * list byte))
+(gv: globals) : environ -> mpred :=
+    EX i : Z, EX cur : val, EX l_cur : val,
+    PROP(0 <= i < Zlength sigma + 1;
+         cur <> nullval;
+         l_cur <> nullval)
+    LOCAL(temp _new new_pointer; 
+          temp _l l;
+          temp _cur cur; 
+          temp _l_cur l_cur; 
+          gvars gv)
+    SEP(malloc_token Ews t_list cur;
+        data_at_ Ews t_list cur;
+        lseg (sublist 0 i sigma) new_pointer cur; 
+        lseg (sublist 0 i sigma) l l_cur;
+        listrep (sublist i (Zlength sigma) sigma) l_cur;
+        mem_mgr gv).
+
+
+Lemma body_list_copy: semax_body Vprog Gprog f_list_copy list_copy_spec.
+Proof.
+  start_function.
+  forward_if(l <> nullval). 
+  { forward. Exists nullval. entailer!. getnw.
+    desc. assert (nullval = nullval) as Trivial by auto.
+    apply LIST_PTR_FACT0 in Trivial.
+    subst.
+    unfold listrep. entailer!.
+  }
+  { forward. entailer!. }
+
+  forward_call(t_list, gv).
+  Intros new_pointer.
+  destruct (eq_dec new_pointer nullval). 
+  { forward_if(new_pointer <> nullval).
+    { forward_call. entailer!. }
+    { forward. entailer!. } 
+    forward. contradiction.
+  }
+
+  forward_if(new_pointer <> nullval).
+  { forward_call. entailer!. }
+  { forward. entailer!. }
+
+  Intros. do 2 forward.
+  
+  forward_loop (
+    list_copy_loop_invariant l new_pointer sigma gv
+  ) break: (
+    PROP()
+    LOCAL(temp _new new_pointer; gvars gv)
+    SEP(listrep sigma new_pointer; listrep sigma l; mem_mgr gv)
+  ).
+  3: { forward. Exists new_pointer. entailer!. }
+  { Exists 0 new_pointer l.
+    entailer!.
+    replace (sublist 0 0 sigma) with ([] : list (Z * list byte)) by list_solve.
+    unfold lseg.
+    replace (sublist 0 (Zlength sigma) sigma) with sigma by list_solve.
+    entailer!.
+  }
+  
+  unfold list_copy_loop_invariant.
+  Intros i cur l_cur.
+  destruct (eq_dec i (Zlength sigma)) as [ | I_is_not_zlength]. 
+  { subst.
+    replace ((sublist (Zlength sigma) (Zlength sigma) sigma)) with ([] : list (Z * list byte)) by list_solve.
+    unfold listrep; fold listrep. 
+    Intros. contradiction.
+  }
+
+replace (sublist i (Zlength sigma) sigma) with 
+  (Znth i sigma :: sublist (i + 1) (Zlength sigma) sigma) by list_solve.
+unfold listrep; fold listrep.
+remember (Znth i sigma) as ith_element eqn:eqn_ith_element.
+destruct ith_element as (shift_i, line_i).
+
+Intros l_cur_tail line_i_pointer.
+do 3 forward.
+forward_call(Ews, line_i, line_i_pointer).
+forward_call((Tarray tschar (Zlength line_i + 1) noattr), gv). {
+  assert (In (shift_i, line_i) sigma) as In_fact. 
+  { rewrite eqn_ith_element. apply Znth_In. lia. }
+
+  assert (Zlength line_i + 1 <= Int.max_unsigned) as Zlength_fact. {
+    remember (fun x : Z * list byte =>
+    0 <= fst x <= Int.max_unsigned /\
+    0 <= Zlength (snd x) + 1 <= Int.max_unsigned) as List_condition.
+    assert (List_condition (shift_i, line_i)) as Ith_condition. 
+    { apply (computable_theorems.Forall_forall1 _ sigma); auto. }
+    rewrite HeqList_condition in Ith_condition.
+    destruct Ith_condition as [shift_condition].
+    simpl in *. lia.
+  }
+
+  unfold sizeof. unfold Ctypes.sizeof.
+  unfold Int.max_unsigned in Zlength_fact. simpl in Zlength_fact.
+  unfold Ptrofs.max_unsigned. simpl.
+  lia.
+}
+
+Intros cur_line_i_pointer.
+destruct (eq_dec cur_line_i_pointer nullval). 
+{ do 2 forward.
+  forward_if(cur_line_i_pointer <> nullval).
+  { forward_call. entailer!. }
+  { forward. entailer!. }
+  forward. contradiction.
+}
+
+Intros. do 2 forward.
+forward_if(cur_line_i_pointer <> nullval).
+{ forward_call. entailer!. }
+{ forward. entailer!. }
+
+do 2 forward.
+forward_call(Ews, Ews, cur_line_i_pointer, Zlength line_i + 1, line_i_pointer, line_i).
+do 2 forward.
+{ entailer!. getnw. desf. }
+
+forward_if(l_cur_tail <> nullval). 
+{ do 2 forward.
+  entailer!.
+  rewrite <- cstringn_equiv.
+  assert (i + 1 = Zlength sigma) as AA. {
+    assert (i + 1 < Zlength sigma \/ i + 1 = Zlength sigma) as BB. lia.
+    destruct BB. {
+      replace (sublist (i + 1) (Zlength sigma) sigma) 
+        with (Znth (i + 1) sigma :: (sublist (i + 2) (Zlength sigma) sigma)) in * by list_solve.
+      unnw.
+      desf.
+      assert( Znth (i + 1) sigma :: sublist (i + 2) (Zlength sigma) sigma = []) as CC by auto.
+      inversion CC.
+    }
+    auto.
+  }
+  rewrite AA.
+  replace (sublist (Zlength sigma) (Zlength sigma) sigma) with ([] : list (Z * list byte)) by list_solve.
+  unfold listrep; fold listrep.
+  
+  entailer!.
+
+  assert (
+    cstring Ews line_i cur_line_i_pointer 
+      * cstring Ews line_i line_i_pointer
+      * malloc_token Ews (Tarray tschar (Zlength line_i + 1) noattr) cur_line_i_pointer
+      * malloc_token Ews t_list cur
+      * data_at Ews t_list (Vint (Int.repr shift_i), (cur_line_i_pointer, Vlong (Int64.repr 0))) cur
+      * lseg (sublist 0 i sigma) new_pointer cur
+      * lseg (sublist 0 i sigma) l l_cur
+      * (emp || malloc_token Ews (Tarray tschar (Zlength line_i + 1) noattr) line_i_pointer)
+      * malloc_token Ews t_list l_cur
+      * data_at Ews t_list (Vint (Int.repr shift_i), (line_i_pointer, nullval)) l_cur
+    |-- 
+    (lseg (sublist 0 i sigma) new_pointer cur *
+    (
+      malloc_token Ews (Tarray tschar (Zlength line_i + 1) noattr) cur_line_i_pointer
+      * cstring Ews line_i cur_line_i_pointer 
+      * malloc_token Ews t_list cur
+      * data_at Ews t_list (Vint (Int.repr shift_i), (cur_line_i_pointer, Vlong (Int64.repr 0))) cur
+    )) * (
+      lseg (sublist 0 i sigma) l l_cur *
+      (
+      (emp || malloc_token Ews (Tarray tschar (Zlength line_i + 1) noattr) line_i_pointer)
+      * cstring Ews line_i line_i_pointer
+      * malloc_token Ews t_list l_cur
+      * data_at Ews t_list (Vint (Int.repr shift_i), (line_i_pointer, nullval)) l_cur
+      )
+    )
+  ) as Trans_step1. 
+  { entailer!. }
+
+  eapply (derives_trans _ _ _); eauto. 
+  apply sepcon_derives. 
+  {
+    assert (sigma = sublist 0 i sigma ++ sublist i (Zlength sigma) sigma) as FF by list_solve.
+    rewrite FF.
+    assert (
+      lseg (sublist 0 i (sublist 0 i sigma ++ sublist i (Zlength sigma) sigma)) new_pointer cur
+       * (malloc_token Ews (Tarray tschar (Zlength line_i + 1) noattr) cur_line_i_pointer
+       * cstring Ews line_i cur_line_i_pointer
+       * malloc_token Ews t_list cur
+       * data_at Ews t_list (Vint (Int.repr shift_i), (cur_line_i_pointer, Vlong (Int64.repr 0))) cur)
+       |-- 
+      lseg (sublist 0 i (sublist 0 i sigma ++ sublist i (Zlength sigma) sigma)) new_pointer cur *
+      listrep [(shift_i, line_i)] cur
+    ) as Trans_step2. {
+      unfold listrep; fold listrep.
+      Exists nullval cur_line_i_pointer.
+      entailer!. apply orp_right2. entailer.
+    }
+
+    eapply (derives_trans _ _ _); eauto.
+    rewrite eqn_ith_element.
+    replace [Znth i sigma] with (sublist i (Zlength sigma) sigma) by list_solve.
+    replace (sublist 0 i sigma ++ sublist i (Zlength sigma) sigma) with sigma at 1 by list_solve.
+    apply lseg_list.
+  }
+  {
+    assert (sigma = sublist 0 i sigma ++ sublist i (Zlength sigma) sigma) as FF by list_solve.
+    rewrite FF.
+    assert (
+      lseg (sublist 0 i (sublist 0 i sigma ++ sublist i (Zlength sigma) sigma)) l l_cur
+        * ((emp || malloc_token Ews (Tarray tschar (Zlength line_i + 1) noattr) line_i_pointer)
+          * cstring Ews line_i line_i_pointer
+          * malloc_token Ews t_list l_cur
+          * data_at Ews t_list (Vint (Int.repr shift_i), (line_i_pointer, nullval)) l_cur)
+      |-- 
+      lseg (sublist 0 i (sublist 0 i sigma ++ sublist i (Zlength sigma) sigma)) l l_cur *
+      listrep [(shift_i, line_i)] l_cur
+    ) as Trans_step2. {
+      unfold listrep; fold listrep.
+      Exists nullval line_i_pointer.
+      entailer!.
+    }
+
+    eapply (derives_trans _ _ _); eauto.
+    rewrite eqn_ith_element.
+    replace [Znth i sigma] with (sublist i (Zlength sigma) sigma) by list_solve.
+    replace (sublist 0 i sigma ++ sublist i (Zlength sigma) sigma) with sigma at 1 by list_solve.
+    apply lseg_list.
+  }
+  }
+  { forward. entailer!. }
+  Intros.
+  forward_call(t_list, gv).
+  Intros cur_tail.
+  do 2 forward.
+  destruct (eq_dec cur_tail nullval). 
+  { forward_if(cur_tail <> nullval).
+    { forward_call. entailer!. }
+    { forward. entailer!. }
+    forward. contradiction.
+  }
+  forward_if(cur_tail <> nullval). 
+  { forward_call. entailer!. }
+  { forward. entailer!. }
+  Intros.
+
+  do 2 forward.
+  Exists (i + 1) cur_tail l_cur_tail.
+  entailer!.
+  rewrite <- cstringn_equiv.
+
+  assert (
+    cstring Ews line_i cur_line_i_pointer * cstring Ews line_i line_i_pointer
+    * malloc_token Ews (Tarray tschar (Zlength line_i + 1) noattr) cur_line_i_pointer
+    * malloc_token Ews t_list cur
+    * data_at Ews t_list (Vint (Int.repr shift_i), (cur_line_i_pointer, cur_tail)) cur
+    * lseg (sublist 0 i sigma) new_pointer cur
+    * lseg (sublist 0 i sigma) l l_cur
+    * (emp || malloc_token Ews (Tarray tschar (Zlength line_i + 1) noattr) line_i_pointer)
+    * malloc_token Ews t_list l_cur
+    * data_at Ews t_list (Vint (Int.repr shift_i), (line_i_pointer, l_cur_tail)) l_cur
+    |--
+    (lseg (sublist 0 i sigma) new_pointer cur
+    * (malloc_token Ews (Tarray tschar (Zlength line_i + 1) noattr) cur_line_i_pointer
+    * cstring Ews line_i cur_line_i_pointer
+    * malloc_token Ews t_list cur
+    * data_at Ews t_list (Vint (Int.repr shift_i), (cur_line_i_pointer, cur_tail)) cur))
+    * (lseg (sublist 0 i sigma) l l_cur
+    * ((emp || malloc_token Ews (Tarray tschar (Zlength line_i + 1) noattr) line_i_pointer)
+    * cstring Ews line_i line_i_pointer
+    * malloc_token Ews t_list l_cur
+    * data_at Ews t_list (Vint (Int.repr shift_i), (line_i_pointer, l_cur_tail)) l_cur))
+  ) as AA by entailer!.
+  
+  eapply (derives_trans _ _ _); eauto.
+  apply sepcon_derives. {
+    clear AA.
+    assert (
+      lseg (sublist 0 i sigma) new_pointer cur
+       * (malloc_token Ews (Tarray tschar (Zlength line_i + 1) noattr) cur_line_i_pointer
+       * cstring Ews line_i cur_line_i_pointer
+       * malloc_token Ews t_list cur
+       * data_at Ews t_list (Vint (Int.repr shift_i), (cur_line_i_pointer, cur_tail)) cur)
+      |-- 
+      lseg (sublist 0 i sigma) new_pointer cur * 
+      lseg (sublist i (i + 1) sigma) cur cur_tail
+    ). 
+    { apply sepcon_derives. entailer.
+      replace (sublist i (i + 1) sigma) with [Znth i sigma] by list_solve.
+      unfold lseg.
+      rewrite <- eqn_ith_element.
+      Exists cur_tail cur_line_i_pointer.
+      entailer!.
+      apply orp_right2. entailer.
+    }
+    eapply (derives_trans _ _ _); eauto.
+    replace (sublist 0 (i + 1) sigma) with (sublist 0 i sigma ++ sublist i (i + 1) sigma) by list_solve.
+    apply lseg_lseg.
+  }
+  { clear AA.
+    assert (
+      lseg (sublist 0 i sigma) l l_cur
+      * ((emp || malloc_token Ews (Tarray tschar (Zlength line_i + 1) noattr) line_i_pointer)
+      * cstring Ews line_i line_i_pointer
+      * malloc_token Ews t_list l_cur
+      * data_at Ews t_list (Vint (Int.repr shift_i), (line_i_pointer, l_cur_tail)) l_cur)
+      |-- 
+      lseg (sublist 0 i sigma) l l_cur * 
+      lseg (sublist i (i + 1) sigma) l_cur l_cur_tail
+    ). {
+      apply sepcon_derives. entailer.
+      replace (sublist i (i + 1) sigma) with [Znth i sigma] by list_solve.
+      unfold lseg.
+      rewrite <- eqn_ith_element.
+      Exists l_cur_tail line_i_pointer.
+      entailer!.
+    }
+    eapply (derives_trans _ _ _); eauto.
+    replace (sublist 0 (i + 1) sigma) with (sublist 0 i sigma ++ sublist i (i + 1) sigma) by list_solve.
+    apply lseg_lseg.
+  }
+Qed.
